theories/iris/logrel/fundamental_kinding.v
@@ -7,6 +7,7 @@ From RichWasm.compiler Require Import prelude module.
 From RichWasm.iris Require Import autowp gc.
 From RichWasm.iris.logrel Require Import relations.
 From Stdlib Require Import Relations.Relation_Operators.
+From stdpp Require Import list.
 
 Set Bullet Behavior "Strict Subproofs".
 Set Default Goal Selector "!".
@@ -24,7 +25,20 @@ Section FundamentalKinding.
     ∀ (T: @semantic_type Σ), 
       T ⊑ T.
   Proof.
-  Admitted.
+    by iIntros (T sv) "H".
+  Qed.
+
+  Lemma semantic_type_le_trans :
+    ∀ (S T U: @semantic_type Σ), 
+      S ⊑ T ->
+      T ⊑ U ->
+      S ⊑ U.
+  Proof.
+    iIntros (S T U Hst Htu sv) "H".
+    iApply Htu.
+    iApply Hst.
+    done.
+  Qed.
 
   Lemma sizity_sized_le_unsized σ :
     sizity_interp (Σ:=Σ) (Sized σ) ⊑ sizity_interp Unsized.
@@ -86,19 +100,137 @@ Section FundamentalKinding.
     subkind_of κ κ' ->
     kind_as_type_interp (Σ := Σ) sr κ ⊑ kind_as_type_interp sr κ'.
   Proof.
-  Admitted.
+    induction 1; cbn; eauto using semantic_type_le_refl.
+    iIntros (sv [(μ' & ws & Hwords & Hsz) Hmem]).
+    iSplit; eauto.
+    iPureIntro.
+    exists μ', ws.
+    split; auto.
+    intros; congruence.
+  Qed.
 
   Lemma rt_subkind_sound κ κ' :
     clos_refl_trans _ subkind_of κ κ' ->
     kind_as_type_interp (Σ := Σ) sr κ ⊑ kind_as_type_interp sr κ'.
   Proof. 
+    intros H.
+    induction H.
+    - by apply subkind_sound.
+    - by apply semantic_type_le_refl.
+    - by eapply semantic_type_le_trans.
+  Qed.
+
+  Lemma subkind_of_subst s__mem s__rep s__size κ κ' :
+    subkind_of κ κ' ->
+    subkind_of (subst_kind s__mem s__rep s__size κ)
+               (subst_kind s__mem s__rep s__size κ').
+  Proof.
+    intros Hle.
+    destruct Hle; constructor.
+  Qed.
+  
+  Lemma rep_ok_subst K ρ :
+    rep_ok K ρ ->
+    forall s__rep,
+      rep_subst_interp K s__rep ->
+      rep_ok kc_empty (subst_representation s__rep ρ).
+  Proof.
+    induction 1; intros; eauto.
   Admitted.
   
-  Lemma has_kind_subst F τ κ s__mem s__rep s__size :
-    has_kind F τ κ ->
-    subst_interp F.(fc_kind_ctx) s__mem s__rep s__size ->
-    has_kind fc_empty (subst_type s__mem s__rep s__size VarT τ) (subst_kind s__mem s__rep s__size κ).
+  Lemma kind_ok_subst K κ :
+    kind_ok K κ ->
+    forall s__mem s__rep s__size,
+      subst_interp K s__mem s__rep s__size ->
+      kind_ok kc_empty (subst_kind s__mem s__rep s__size κ).
   Proof.
+    unfold subst_interp.
+    induction 1; intros * (Hmem & Hrep & Hsz).
+    - constructor.
+      eapply rep_ok_subst; eauto.
+    - constructor.
+      + admit.
+      + admit.
+  Admitted.
+  
+  Ltac fold_subst :=
+    fold subst_type subst_size subst_representation subst_function_type.
+  
+  Lemma has_kind_subst F τ κ :
+    has_kind F τ κ ->
+    ∀ s__mem s__rep s__size,
+        subst_interp F.(fc_kind_ctx) s__mem s__rep s__size ->
+        has_kind 
+          (fc_clear_kind (subst_function_ctx s__mem s__rep s__size VarT F))
+          (subst_type s__mem s__rep s__size VarT τ)
+          (subst_kind s__mem s__rep s__size κ).
+  Proof.
+    induction 1 using has_kind_ind'; intros s__mem s__rep s__size Hsubst; try solve [econstructor; eauto].
+    - eapply IHhas_kind in Hsubst.
+      econstructor; eauto using subkind_of_subst.
+    - cbn.
+      eapply KVar.
+      + cbn.
+        by rewrite list_lookup_fmap H.
+      + by eapply kind_ok_subst.
+    - eapply KSumVal.
+      fold_subst.
+      apply Forall2_fmap; eapply Forall2_impl; eauto.
+    - eapply KSumMem.
+      { admit. }
+      apply Forall2_fmap; eapply Forall2_impl; eauto.
+    - eapply KSumMemSized.
+      { admit. }
+      apply Forall2_fmap; eapply Forall2_impl; eauto.
+    - eapply KProdVal.
+      fold_subst.
+      apply Forall2_fmap; eapply Forall2_impl; eauto.
+    - eapply KProdMem.
+      { admit. }
+      fold_subst.
+      apply Forall2_fmap; eapply Forall2_impl; eauto.
+    - eapply KProdMemSized.
+      { admit. }
+      fold_subst.
+      apply Forall2_fmap; eapply Forall2_impl; eauto.
+    - eapply KCodeRef.
+      fold_subst.
+      admit.
+    - eapply KRep.
+      { admit. }
+      fold_subst.
+      eauto.
+    - eapply KPad.
+      { admit. }
+      fold_subst.
+      eauto.
+    - eapply KSer.
+      { admit. }
+      fold_subst; eauto.
+    - eapply KRec.
+      fold_subst.
+      admit.
+    - eapply KExistsMem.
+      { eapply kind_ok_subst; eauto. }
+      fold_subst.
+      admit.
+    - eapply KExistsRep.
+      { eapply kind_ok_subst; eauto. }
+      fold_subst.
+      set (s__mem' := up_representation_memory s__mem).
+      set (s__rep' := up_representation_representation s__rep).
+      set (s__size' := up_representation_size s__size).
+      set (F' := RecordSet.set _ _ _) in *.
+      set (F'' := RecordSet.set _ _ _).
+      erewrite ext_type; first last.
+      + intros i.
+        rewrite upId_representation_type; eauto.
+      + reflexivity.
+      + reflexivity.
+      + reflexivity.
+      + admit.
+    - admit.
+    - admit.
   Admitted.
 
   Theorem kinding_refinement F s__mem s__rep s__size se τ κ : 
@@ -114,8 +246,13 @@ Section FundamentalKinding.
     rewrite value_interp_eq.
     iDestruct "Hval" as "(%κ' & %Htyk & Hinterp & _)".
     eapply has_kind_subst in Hhas_kind; eauto.
-    eapply (type_kind_has_kind_agree fc_empty) in Hhas_kind; eauto.
-    iApply rt_subkind_sound; eauto.
+    eapply type_kind_has_kind_agree in Hhas_kind; cbn; eauto.
+  Admitted.
+  
+  Instance kind_as_type_persistent κ sv :
+    @Persistent (iProp Σ) (kind_as_type_interp sr κ sv).
+  Proof.
+    destruct κ; typeclasses eauto.
   Qed.
 
   Theorem kinding_copyable F s__mem s__rep s__size se τ ρ χ δ : 
@@ -128,53 +265,75 @@ Section FundamentalKinding.
     revert Heqκ.
     revert ρ χ δ.
     induction Hkind; intros ? ? ? Hκeq; rewrite -> Hκeq in *;
-      iIntros "[%Hsubst Henv]"; unfold copyability_interp;
-      try (subst κ; inversion Hκeq; subst).
-    - subst.
-      admit.
-    - assert (Ht: exists Tt, se !! t = Some Tt) by admit.
-      destruct Ht as [Tt Ht].
-      eapply big_sepL2_lookup_acc in H; eauto.
-      iPoseProof (H with "Henv") as "[H _]".
-      iDestruct "H" as "[%Ht' Ht'']".
-      remember (value_interp _ _ _ _) as T.
-      assert (T ≡ Tt).
-      {
-        rewrite HeqT.
-        cbn.
-        intros x.
-        rewrite value_interp_eq.
-        cbn.
-        rewrite Ht; cbn.
+      iIntros "[%Hsubst Henv]"; try subst κ; try subst κ'.
+    - inversion H; subst; eauto.
+      + specialize (IHHkind _ _ _ eq_refl).
+        cbn in IHHkind.
         admit.
-      }
+      + iApply IHHkind; eauto.
+        by iFrame.
+      + iApply IHHkind; eauto.
+        by iFrame.
+    - simpl subst_type.
+      unfold copyability_interp.
+      destruct χ; simpl.
+      + done.
+      + unfold explicit_copy_spec.
+        iIntros.
+        rewrite value_interp_eq; cbn.
+        admit.
+      + setoid_rewrite value_interp_eq; cbn.
+        admit.
+    - unfold copyability_interp; inversion Hκeq; subst; eauto.
+      cbn.
+      iIntros "%sv !%".
+      rewrite value_interp_eq; cbn.
+      eapply bi.exist_persistent; intros κ.
+      destruct κ; cbn; typeclasses eauto.
+    - unfold copyability_interp; inversion Hκeq; subst; eauto.
+      iIntros "%sv !%".
+      rewrite value_interp_eq; cbn.
+      eapply bi.exist_persistent; intros κ.
+      destruct κ; cbn; typeclasses eauto.
+    - unfold copyability_interp; inversion Hκeq; subst; eauto.
+      iIntros "%sv !%".
+      rewrite value_interp_eq; cbn; typeclasses eauto.
+    - unfold copyability_interp; inversion Hκeq; subst; eauto.
+      iIntros "%sv !%".
+      rewrite value_interp_eq; cbn; typeclasses eauto.
+    - unfold copyability_interp; inversion Hκeq; subst; eauto.
+      iIntros "%sv !%".
+      rewrite value_interp_eq; cbn; typeclasses eauto.
+    - admit. (* sums *)
+    - inversion Hκeq; subst; eauto.
+    - inversion Hκeq; subst; eauto.
+    - admit. (* products *)
+    - inversion Hκeq; subst; eauto.
+    - inversion Hκeq; subst; eauto.
+    - inversion Hκeq; subst; eauto.
+    - inversion Hκeq; subst; eauto.
+    - admit. (* refs *)
+    - inversion Hκeq; subst.
+    - admit. (* coderef *)
+    - inversion Hκeq; subst; cbn; eauto.
+      destruct χ0; cbn.
+      + done.
+      + unfold explicit_copy_spec.
+        iIntros.
+        rewrite value_interp_eq; simpl.
+        admit.
+      + setoid_rewrite value_interp_eq; cbn.
+        iPoseProof (IHHkind _ _ _ eq_refl) as "IH".
+        iSpecialize ("IH" with "[Henv]"); [by iFrame|].
+        cbn.
+        iPoseProof "IH" as "%IH".
+        iIntros "!% %sv".
+        repeat ((eapply bi.exist_persistent; intros) 
+                || eapply bi.sep_persistent
+                || typeclasses eauto).
+    - cbn in *. 
       admit.
-    - iIntros "%sv !%".
-      rewrite value_interp_eq; cbn.
-      eapply bi.exist_persistent; intros κ.
-      destruct κ; cbn; typeclasses eauto.
-    - iIntros "%sv !%".
-      rewrite value_interp_eq; cbn.
-      eapply bi.exist_persistent; intros κ.
-      destruct κ; cbn; typeclasses eauto.
-    - iIntros "%sv !%".
-      rewrite value_interp_eq; cbn.
-      eapply bi.exist_persistent; intros κ.
-      destruct κ; cbn; typeclasses eauto.
-    - iIntros "%sv !%".
-      rewrite value_interp_eq; cbn.
-      eapply bi.exist_persistent; intros κ.
-      destruct κ; cbn; typeclasses eauto.
-    - admit.
-    - admit.
-    - admit. (* Product case! *)
-    - auto.
-    - auto.
-    - iIntros (fr ιs vs es) "%Hevalrep %Hcopyop Hfr Hrun Hval".
-      unfold is_copy_operation in Hcopyop.
-      admit.
-    - admit. (* function type stuff...? *)
-    - admit.
+    - unfold copyability_interp; inversion Hκeq; subst; eauto.
     - admit.
     - admit.
     - admit.
